intermediate2/Zeta.Intermediate.Verifier.fst
@@ -1,8 +1,8 @@
 module Zeta.Intermediate.Verifier
 
-#push-options "--fuel 0 --ifuel 1 --z3rlimit_factor 2 --query_stats"
+#push-options "--z3rlimit_factor 3 --query_stats"
 
-let vaddm #vcfg (r:record vcfg.app) (s:slot_id vcfg)  (s':slot_id vcfg) (vs: vtls_t vcfg {vs.valid}):
+let addm #vcfg (r:record vcfg.app) (s:slot_id vcfg)  (s':slot_id vcfg) (vs: vtls_t vcfg {vs.valid}):
   (vs': vtls_t vcfg {let a = AMP s r s' vs in
                    addm_precond a /\ addm_postcond a vs' \/
                    ~(addm_precond a) /\ ~vs'.valid}) =
@@ -61,3 +61,239 @@ let vaddm #vcfg (r:record vcfg.app) (s:slot_id vcfg)  (s':slot_id vcfg) (vs: vtl
             update_thread_store vs st
 
 #pop-options
+
+(* does a slot contain an app key *)
+let contains_app_key (#vcfg:_) (st: vstore vcfg) (s: slot_id vcfg)
+  = inuse_slot st s &&
+    AppK? (stored_key st s)
+
+(* a sequence of base keys contain only appln keys *)
+let contains_only_app_keys (#vcfg:_) (st: vstore vcfg) (ss: S.seq (slot_id vcfg))
+  = forall i. contains_app_key st (S.index ss i)
+
+let contains_only_app_keys_comp (#vcfg:_) (st: vstore vcfg) (ss: S.seq (slot_id vcfg))
+  : b:bool {b <==> contains_only_app_keys st ss}
+  = let open Zeta.SeqIdx in
+    not (exists_elems_with_prop_comp (fun s -> not (contains_app_key st s)) ss)
+
+let puts (#vcfg:_)
+  (vs: vtls_t vcfg{vs.valid})
+  (ss: S.seq (slot_id vcfg))
+  (ws: S.seq (app_value_nullable vcfg.app.adm))
+  : vs': vtls_t vcfg{vs'.valid}
+  = let st = puts_store vs.st ss ws in
+    update_thread_store vs st
+
+let clock_is_monotonic
+  (#vcfg:_)
+  (e: GV.verifier_log_entry (int_verifier_spec_base vcfg))
+  (vs: vtls_t vcfg)
+  : Lemma (ensures (let vs_post = GV.verify_step e vs in
+                    vs_post.valid ==> vs.clock `ts_leq` vs_post.clock))
+  = ()
+
+let lemma_int_verifier_clock_monotonic_prop (vcfg:_)
+  : Lemma (ensures (GV.clock_monotonic_prop (int_verifier_spec_base vcfg)))
+  = FStar.Classical.forall_intro_2 (clock_is_monotonic #vcfg)
+
+let thread_id_is_constant
+  (#vcfg:_)
+  (e: GV.verifier_log_entry (int_verifier_spec_base vcfg))
+  (vs: vtls_t vcfg)
+  : Lemma (ensures (let vs_post = GV.verify_step e vs in
+                    vs.tid = vs_post.tid))
+  = ()
+
+let lemma_int_verifier_thread_id_const_prop (vcfg:_)
+  : Lemma (ensures (GV.thread_id_constant_prop (int_verifier_spec_base vcfg)))
+  = FStar.Classical.forall_intro_2 (thread_id_is_constant #vcfg)
+
+let evict_prop
+  (#vcfg:_)
+  (e: GV.verifier_log_entry (int_verifier_spec_base vcfg))
+  (vs: vtls_t vcfg)
+  : Lemma (ensures (let vs_post = GV.verify_step e vs in
+                    GV.is_evict e ==>
+                    vs_post.valid ==>
+                    inuse_slot vs.st (GV.evict_slot e) /\
+                    empty_slot vs_post.st (GV.evict_slot e)))
+  = ()
+
+let lemma_int_verifier_evict_prop (vcfg:_)
+  : Lemma (ensures (GV.evict_prop (int_verifier_spec_base vcfg)))
+  = FStar.Classical.forall_intro_2 (evict_prop #vcfg)
+
+let add_prop
+  (#vcfg:_)
+  (e: GV.verifier_log_entry (int_verifier_spec_base vcfg))
+  (vs: vtls_t vcfg)
+  : Lemma (ensures (let vs_post = GV.verify_step e vs in
+                    GV.is_add e ==>
+                    vs_post.valid ==>
+                    (empty_slot vs.st (GV.add_slot e)) /\
+                    inuse_slot vs_post.st (GV.add_slot e)))
+  = ()
+
+let lemma_int_verifier_add_prop (vcfg:_)
+  : Lemma (ensures (GV.add_prop (int_verifier_spec_base vcfg)))
+  = FStar.Classical.forall_intro_2 (add_prop #vcfg)
+
+let addb_prop
+  (#vcfg:_)
+  (e: GV.verifier_log_entry (int_verifier_spec_base vcfg))
+  (vs: vtls_t vcfg)
+  : Lemma (ensures (let vs_post = GV.verify_step e vs in
+                    GV.is_blum_add e ==>
+                    vs_post.valid ==>
+                    GV.blum_add_timestamp e `ts_lt` vs_post.clock))
+  = ()
+
+let lemma_int_verifier_addb_prop (vcfg:_)
+  : Lemma (ensures (GV.addb_prop (int_verifier_spec_base vcfg)))
+  = FStar.Classical.forall_intro_2 (addb_prop #vcfg)
+
+let evictb_prop
+  (#vcfg:_)
+  (e: GV.verifier_log_entry (int_verifier_spec_base vcfg))
+  (vs: vtls_t vcfg)
+  : Lemma (ensures (let vs_post = GV.verify_step e vs in
+                    GV.is_blum_evict e ==>
+                    vs_post.valid ==>
+                    (vs.clock `ts_lt` vs_post.clock /\
+                     vs_post.clock = GV.blum_evict_timestamp e)))
+  = ()
+
+let lemma_int_verifier_evictb_prop (vcfg:_)
+  : Lemma (ensures (GV.evictb_prop (int_verifier_spec_base vcfg)))
+  = FStar.Classical.forall_intro_2 (evictb_prop #vcfg)
+
+let lemma_int_verifier (vcfg: verifier_config)
+  : Lemma (ensures (GV.clock_monotonic_prop (int_verifier_spec_base vcfg) /\
+                    GV.thread_id_constant_prop (int_verifier_spec_base vcfg) /\
+                    GV.evict_prop (int_verifier_spec_base vcfg) /\
+                    GV.add_prop (int_verifier_spec_base vcfg) /\
+                    GV.addb_prop (int_verifier_spec_base vcfg) /\
+                    GV.evictb_prop (int_verifier_spec_base vcfg)))
+  = lemma_int_verifier_clock_monotonic_prop vcfg;
+    lemma_int_verifier_thread_id_const_prop vcfg;
+    lemma_int_verifier_evict_prop vcfg;
+    lemma_int_verifier_add_prop vcfg;
+    lemma_int_verifier_addb_prop vcfg;
+    lemma_int_verifier_evictb_prop vcfg
+
+let lemma_addm_props (#vcfg:_)
+                     (vs':vtls_t vcfg{vs'.valid})
+                     (e:logS_entry _{GV.AddM? e}):
+  Lemma (requires ((GV.verify_step e vs').valid))
+        (ensures (let GV.AddM (gk,gv) s s' = e in
+                  let st' = vs'.st in
+                  let k = to_base_key gk in
+                  inuse_slot st' s' /\
+                  (let k' = stored_base_key st' s' in
+                   is_proper_desc k k' /\
+                   is_merkle_key k' /\
+                   (let mv' = to_merkle_value (stored_value st' s') in
+                    let d = desc_dir k k' in
+                    (Merkle.points_to_none mv' d ||
+                     is_desc (Merkle.pointed_key mv' d) k)))))
+  = let GV.AddM (gk,gv) s s' = e in
+    let st' = vs'.st in
+    let k = to_base_key gk in
+    let k' = stored_base_key st' s' in
+    assert(is_proper_desc k k');
+    assert(is_merkle_key k');
+    let mv' = to_merkle_value (stored_value st' s') in
+    let d = desc_dir k k' in
+    let dh' = desc_hash mv' d in
+    match dh' with
+    | Empty -> ()
+    | Desc k2 _ _  ->
+      if k2 = k then lemma_desc_reflexive k
+
+let lemma_runapp_preserves_ismap
+      (#vcfg:_)
+      (vs:vtls_t vcfg{vs.valid})
+      (e:logS_entry _{GV.is_appfn e})
+  : Lemma (requires (is_map (vs.st)))
+          (ensures (let vs_ = GV.verify_step e vs in
+                    vs_.valid ==> is_map vs_.st))
+  = ()
+
+(* if the key is not present in store and store is a map, then store remains a map after add *)
+let lemma_vaddm_preserves_ismap_new_key
+      (#vcfg:_)
+      (vs:vtls_t vcfg{vs.valid})
+      (e:logS_entry _{GV.AddM? e})
+  : Lemma (requires (let st = vs.st in
+                     let GV.AddM (gk,gv) _  _ = e in
+                     let k = to_base_key gk in
+                     is_map st /\ not (store_contains_key st k)))
+          (ensures (let vs_ = GV.verify_step e vs in
+                    vs_.valid ==> is_map vs_.st))
+  = ()
+
+let lemma_vaddb_preserves_ismap_new_key
+      (#vcfg:_)
+      (vs:vtls_t vcfg{vs.valid})
+      (e:logS_entry _{GV.AddB? e})
+  : Lemma (requires (let st = vs.st in
+                     let GV.AddB (gk,_) _ _ _ = e in
+                     let k = to_base_key gk in
+                     is_map st /\ not (store_contains_key st k)))
+          (ensures (let vs_ = GV.verify_step e vs in
+                    vs_.valid ==> is_map vs_.st))
+  = ()
+
+let lemma_evictb_preserves_ismap
+      (#vcfg:_)
+      (vs:vtls_t vcfg{vs.valid})
+      (e:logS_entry _{GV.EvictB? e})
+  : Lemma (requires (is_map vs.st))
+          (ensures (let vs_ = GV.verify_step e vs in
+                    vs_.valid ==> is_map vs_.st))
+  = ()
+
+let lemma_evictm_preserves_ismap
+      (#vcfg:_)
+      (vs:vtls_t vcfg{vs.valid})
+      (e:logS_entry _{GV.EvictM? e})
+  : Lemma (requires (is_map vs.st))
+          (ensures (let vs_ = GV.verify_step e vs in
+                    vs_.valid ==> is_map vs_.st))
+  = ()
+
+let lemma_evictbm_preserves_ismap
+      (#vcfg:_)
+      (vs:vtls_t vcfg{vs.valid})
+      (e:logS_entry _{GV.EvictBM? e})
+  : Lemma (requires (is_map vs.st))
+          (ensures (let vs_ = GV.verify_step e vs in
+                    vs_.valid ==> is_map vs_.st))
+  = ()
+
+let lemma_nextepoch_preserves_ismap
+      (#vcfg:_)
+      (vs:vtls_t vcfg{vs.valid})
+  : Lemma (requires (is_map vs.st))
+          (ensures (let intspec = int_verifier_spec vcfg in
+                    let vs_: vtls_t vcfg = GV.verify_step #intspec GV.NextEpoch vs in
+                    vs_.valid ==> is_map vs_.st))
+  = ()
+
+let lemma_verifyepoch_preserves_ismap
+      (#vcfg:_)
+      (vs:vtls_t vcfg{vs.valid})
+  : Lemma (requires (is_map vs.st))
+          (ensures (let intspec = int_verifier_spec vcfg in
+                    let vs_: vtls_t vcfg = GV.verify_step #intspec GV.VerifyEpoch vs in
+                    vs_.valid ==> is_map vs_.st))
+  = ()
+
+let lemma_verifiable_implies_slot_is_merkle_points_to (#vcfg:_)
+                                                      (vs:vtls_t vcfg)
+                                                      (e: logS_entry _):
+  Lemma (requires (vs.valid /\ slot_points_to_is_merkle_points_to vs.st /\
+                   (GV.verify_step e vs).valid))
+        (ensures (let vs_ = GV.verify_step e vs in
+                  slot_points_to_is_merkle_points_to vs_.st))
+  = admit()
